theories/ordinals/Ackermann/fol.v
@@ -723,3 +723,4 @@ Arguments equal {L} _ _.
 Arguments existH {L} _ _.
 Arguments var {L} _.
 Arguments atomic {L} _ _.
+Arguments apply {L} _ _.
