theories/ordinals/Ackermann/folLogic.v
@@ -14,7 +14,6 @@ Let Formulas := Formulas L.
 Let System := System L.
 Let Term := Term L.
 Let Terms := Terms L.
-Let apply := apply L.
 Let ifThenElseH := ifThenElseH L.
 Let Prf := Prf L.
 Let SysPrf := SysPrf L.
